SP.v
@@ -7,6 +7,7 @@ Module SPBase (P X V E B R:DecType) (Ev:Eval E X V V) (BEv:Eval B X V Bool).
 
 Module Export PSt := LState V X.
 Module Export CSt := GState P V X.
+Module Export TL := TransitionLabels P V X R.
 
 Module Bdec := DecidableType B.
 Module Edec := DecidableType E.
@@ -27,28 +28,163 @@ Definition beval := BEv.eval.
 Definition eval_on_state (e:Expr) (s:State) (p:Pid) : Value := eval e (s p).
 Definition beval_on_state (b:BExpr) (s:State) (p:Pid) : bool := beval b (s p).
 
-
 Section Syntax.
+
+(** ** Syntax of processes *)
 
 Inductive Behaviour : Type :=
 | End : Behaviour
 | Send : Pid -> Expr -> Behaviour -> Behaviour
 | Recv : Pid -> Var -> Behaviour -> Behaviour
 | Sel : Pid -> Label -> Behaviour -> Behaviour
-| Branching : Pid -> (Label -> option Behaviour) -> Behaviour
+| Branching : Pid -> list (Label * Behaviour) -> Behaviour
 | Cond : BExpr -> Behaviour -> Behaviour -> Behaviour
 | Call : RecVar -> Behaviour
 .
 
-Definition Branch : Type := option Behaviour.
+Definition Cases := list (Label*Behaviour).
 
-(** Equality of behaviours is not decidable because of branching... *)
-Lemma Behaviour_eq_End_dec : forall (b:Behaviour), {b=End} + {b<>End}.
+(** Informally, we think of [Branching] as a partial function from labels to 
+  behaviours. There are several possible ways of formalizing this; the choice we
+  make corresponds closely to the notation in choreography papers - there is a
+  well-formedness assumption that no label occurs twice in the list. *)
+
+(** In order to do induction on behaviours, WTF?????? *)
+
+Fixpoint depth (B:Behaviour) : nat :=
+match B with
+ | Send p e B' => 1 + depth B'
+ | Recv p x B' => 1 + depth B'
+ | Sel p l B' => 1 + depth B'
+ | Branching p c => 1 + list_max (map (fun p => match p with (_,B') => depth B' end) c)
+ | Cond b B1 B2 => 1 + Nat.max (depth B1) (depth B2)
+ | Call X => 1
+ | End => 1
+end.
+
+Theorem Behaviour_ind' :
+  forall P:Behaviour -> Prop,
+    P End ->
+    (forall (p:Pid) (e:Expr) (B:Behaviour), P B -> P (Send p e B)) ->
+    (forall (p:Pid) (v:Var) (B:Behaviour), P B -> P (Recv p v B)) ->
+    (forall (p:Pid) (l:Label) (B:Behaviour), P B -> P (Sel p l B)) ->
+    (forall (p:Pid) (c:Cases), (forall (l:Label) (B:Behaviour), In (l,B) c -> P B) -> P (Branching p c)) ->
+    (forall (b:BExpr) (B1 B2:Behaviour), P B1 -> P B2 -> P (Cond b B1 B2)) ->
+    (forall (X:RecVar), P (Call X)) ->
+    forall B:Behaviour, P B.
 Proof.
-induction b; auto; right; discriminate.
+intros.
+revert B.
+assert (forall d B, depth B <= d -> P B).
+2: eauto.
+induction d; intros; case_eq B; intros; auto; rewrite H7 in H6; try (exfalso; inversion H6; fail); auto with arith.
++ clear H H0 H1 H2 H4 H5 H7 B.
+  apply H3.
+  intros; apply IHd.
+  simpl in H6. apply le_S_n in H6.
+  rewrite list_max_le, Forall_forall in H6.
+  apply in_map with (f:=fun p:Label*Behaviour => let (_,B):=p in depth B) in H.
+  auto.
++ apply H4; apply IHd; simpl in H; apply le_S_n in H6.
+  - etransitivity. eapply Nat.le_max_l. eauto.
+  - etransitivity. eapply Nat.le_max_r. eauto.
 Qed.
 
+Theorem Behaviour_rec' :
+  forall P:Behaviour -> Type,
+    P End ->
+    (forall (p:Pid) (e:Expr) (B:Behaviour), P B -> P (Send p e B)) ->
+    (forall (p:Pid) (v:Var) (B:Behaviour), P B -> P (Recv p v B)) ->
+    (forall (p:Pid) (l:Label) (B:Behaviour), P B -> P (Sel p l B)) ->
+    (forall (p:Pid) (c:Cases), (forall (l:Label) (B:Behaviour), In (l,B) c -> P B) -> P (Branching p c)) ->
+    (forall (b:BExpr) (B1 B2:Behaviour), P B1 -> P B2 -> P (Cond b B1 B2)) ->
+    (forall (X:RecVar), P (Call X)) ->
+    forall B:Behaviour, P B.
+Proof.
+intros.
+revert B.
+assert (forall d B, depth B <= d -> P B).
+2: eauto.
+induction d; intros; case_eq B; intros; auto; rewrite H0 in H; try (exfalso; inversion H; fail); auto with arith.
++ apply X3.
+  intros; apply IHd.
+  simpl in H. apply le_S_n in H.
+  rewrite list_max_le, Forall_forall in H.
+  apply in_map with (f:=fun p:Label*Behaviour => let (_,B):=p in depth B) in H1.
+  auto.
++ apply X4; apply IHd; simpl in H; apply le_S_n in H.
+  - etransitivity. eapply Nat.le_max_l. eauto.
+  - etransitivity. eapply Nat.le_max_r. eauto.
+Defined.
+
+(** Equality of behaviours is decidable. We are using the fact that equality on labels is decidable. *)
+Lemma Behaviour_eq_dec : forall (B B':Behaviour), {B=B'} + {B<>B'}.
+Proof.
+induction B using Behaviour_rec'; induction B' using Behaviour_rec'; auto;
+  try (right; discriminate).
++ case (P.eq_dec p p0); intros.
+  2: right; intro; inversion H; auto.
+  case (E.eq_dec e e0); intros.
+  2: right; intro; inversion H; auto.
+  elim (IHB B'); intros.
+  2: right; intro; inversion H; auto.
+  rewrite e1, e2, a; auto.
++ case (P.eq_dec p p0); intros.
+  2: right; intro; inversion H; auto.
+  case (X.eq_dec v v0); intros.
+  2: right; intro; inversion H; auto.
+  elim (IHB B'); intros.
+  2: right; intro; inversion H; auto.
+  rewrite e, e0, a; auto.
++ case (P.eq_dec p p0); intros.
+  2: right; intro; inversion H; auto.
+  case (eq_label_dec l l0); intros.
+  2: right; intro; inversion H; auto.
+  elim (IHB B'); intros.
+  2: right; intro; inversion H; auto.
+  rewrite e, e0, a; auto.
++ case (P.eq_dec p p0); intros.
+  2: right; intro; inversion H; auto.
+  assert ({c=c0}+{c<>c0}).
+  - clear e X0 p0. revert c X; induction c0; intros.
+    case c; auto. right; discriminate.
+    case_eq c. right; discriminate.
+    intros. induction p0. rename a0 into l1, b into B1.
+    induction a. rename a into l2, b into B2.
+    case (eq_label_dec l1 l2); intros.
+    2: right; intro; inversion H0; auto.
+    elim (X l1 B1) with B2; intros.
+    2: right; intro; inversion H0; auto.
+    2: rewrite H; simpl; auto.
+    elim (IHc0 l); intros.
+    2: right; intro; inversion H0; auto.
+    rewrite e, a, a0; auto.
+    apply X with l0. rewrite H; right; auto.
+  - inversion_clear H.
+    2: right; intro; inversion H; auto.
+    rewrite e, H0; auto.
++ case (B.eq_dec b b0); intros.
+  2: right; intro; inversion H; auto.
+  case (IHB1 B'1); intros.
+  2: right; intro; inversion H; auto.
+  elim (IHB2 B'2); intros.
+  2: right; intro; inversion H; auto.
+  rewrite e, e0, a; auto.
++ case (R.eq_dec X X0); intros.
+  2: right; intro; inversion H; auto.
+  rewrite e; auto.
+Qed.
+
+Lemma Behaviour_eq_End_dec : forall (b:Behaviour), {b=End} + {b<>End}.
+Proof. intros; apply Behaviour_eq_dec. Qed.
+
+(** ** Networks
+  Networks are maps from process names to behaviours.
+*)
+
 Definition Network := Pid -> Behaviour.
+
+(** A lot of definitions are parameterised on process lists, for decidability. *)
 
 Definition within_ps (ps:list Pid) (N:Network) :=
   forall p, ~In p ps -> N p = End.
@@ -73,6 +209,8 @@ Qed.
 
 Definition finite_support (N:Network) := exists ps, within_ps ps N.
 
+(** Network equality *)
+
 Definition Network_eq (N N':Network) : Prop := forall p, N p = N' p.
 
 Lemma Network_eq_within_ps : forall ps N N',
@@ -87,12 +225,7 @@ elim (In_dec P.eq_dec p ps); intros.
 + rewrite H0; auto.
 Qed.
 
-(*
-Lemma Network_eq_within_ps_dec : forall ps N N', within_ps ps N -> within_ps ps N' ->
-  {Network_eq N N'}+{~Network_eq N N'}.
-Proof.
-intros.
-*)
+(** Syntactic constructors for building networks as lists *)
 
 Definition EmptyNet : Network := fun _ => End.
 
@@ -101,6 +234,9 @@ Proof. red; auto. Qed.
 
 Lemma EmptyNet_finite_supp : finite_support EmptyNet.
 Proof. exists nil. apply EmptyNet_within_ps. Qed.
+
+Definition Process (p:Pid) (B:Behaviour) : Network :=
+  fun p' => if (Pid_dec p' p) then B else End.
 
 Definition Par (N N':Network) :=
   fun p => if (Behaviour_eq_End_dec (N p)) then N' p else N p.
@@ -118,6 +254,17 @@ intros.
 unfold Par. elim Behaviour_eq_End_dec; auto.
 intro. elim b; auto.
 Qed.
+
+Lemma Par_assoc : forall N N' N'',
+  Network_eq (Par N (Par N' N'')) (Par (Par N N') N'').
+Proof.
+red; intros.
+unfold Par.
+do 2 elim Behaviour_eq_End_dec; intros; auto.
+elim b; auto.
+Qed.
+
+(** If two networks do not share any running processes, then their parallel composition is symmetric. *)
 
 Definition Network_disjoint (N N':Network) :=
   forall p, N p = End \/ N' p = End.
@@ -140,17 +287,80 @@ do 2 elim Behaviour_eq_End_dec; intros; auto.
   elim (H p); auto.
 Qed.
 
-Lemma Par_assoc : forall N N' N'',
-  Network_eq (Par N (Par N' N'')) (Par (Par N N') N'').
+(** We can also remove a process from a network. *)
+
+Definition Network_rm (N:Network) (p:Pid) :=
+  fun r => if (Pid_dec r p) then End else N r.
+
+Lemma Network_rm_add :
+  forall N p, Network_eq N (Par (Network_rm N p) (Process p (N p))).
 Proof.
-red; intros.
-unfold Par.
-do 2 elim Behaviour_eq_End_dec; intros; auto.
-elim b; auto.
+intros.
+red. unfold Network_rm, Process, Par. intro.
+case_eq (Pid_dec p0 p); intros.
++ rewrite Pdec.eqb_eq in H. rewrite H.
+  elim Behaviour_eq_End_dec; auto.
+  intro H'. contradiction.
++ elim Behaviour_eq_End_dec; auto.
 Qed.
 
-Definition Process (p:Pid) (b:Behaviour) : Network :=
-  fun p' => if (Pid_dec p' p) then b else End.
+Lemma Network_rm_eq : forall N N', Network_eq N N' ->
+  forall p, Network_eq (Network_rm N p) (Network_rm N' p).
+Proof.
+red; intros. unfold Network_rm.
+case_eq (Pid_dec p0 p); auto.
+Qed.
+
+Lemma Network_rm_within_ps : forall N p ps,
+  within_ps (p::ps) N -> within_ps ps (Network_rm N p).
+Proof.
+red; intros. unfold Network_rm.
+case_eq (Pid_dec p0 p); auto.
+intro; apply H; auto. intro; apply H0; auto.
+inversion_clear H2; auto. rewrite H3 in H1; rewrite Pdec.eqb_neq in H1.
+elim H1; auto.
+Qed.
+
+(* Generalisation of the above to lists of processes. *)
+
+Definition Network_rm_ps (N:Network) (ps:list Pid) :=
+  fun r => if (in_dec P.eq_dec r ps) then End else N r.
+
+Definition Network_res_ps (N:Network) (ps:list Pid) :=
+  fun r => if (in_dec P.eq_dec r ps) then N r else End.
+
+Lemma Network_rm_res_ps :
+  forall N ps, Network_eq N (Par (Network_rm_ps N ps) (Network_res_ps N ps)).
+Proof.
+intros.
+red. unfold Network_rm_ps, Network_res_ps, Par. intro.
+case_eq (in_dec P.eq_dec p ps); intros.
++ elim Behaviour_eq_End_dec; auto.
+  intro. contradiction.
++ elim Behaviour_eq_End_dec; auto.
+Qed.
+
+(** This construction makes the following lemma easier to prove. *)
+Lemma Network_eq_within_ps_dec : forall ps N N', within_ps ps N -> within_ps ps N' ->
+  {Network_eq N N'}+{~Network_eq N N'}.
+Proof.
+induction ps; intros.
++ left. intro. rewrite H, H0; auto.
++ elim (Behaviour_eq_dec (N a) (N' a)); intros.
+  2: right; intro; auto.
+  elim (IHps (Network_rm N a) (Network_rm N' a)); intros;
+  try (apply Network_rm_within_ps; auto).
+  - left; intro.
+    case (P.eq_dec p a); intro. rewrite e; auto.
+    generalize (a1 p).
+    rewrite <- Pdec.eqb_neq in n. fold Pid_dec in n.
+    unfold Network_rm; rewrite n; auto.
+  - right; intro.
+    apply b; intro.
+    apply Network_rm_eq; auto.
+Qed.
+
+(** Programs in SP are pairs, like choreography programs in MC. *)
 
 Record Program : Type :=
   { Procedures : RecVar -> Behaviour;
@@ -158,6 +368,7 @@ Record Program : Type :=
 
 End Syntax.
 
+Declare Scope SP_scope.
 Delimit Scope SP_scope with SP.
 
 Bind Scope SP_scope with Behaviour.
@@ -168,7 +379,7 @@ Notation "p [ B ]" := (Process p B) (at level 201, no associativity) : SP_scope.
 Notation "p ! e ; B" := (Send p e B) (at level 60, e at level 9, right associativity) : SP_scope.
 Notation "p ? xx ; B" := (Recv p xx B) (at level 60, right associativity) : SP_scope.
 Notation "p (+) l ; B" := (Sel p l B) (at level 49, l at level 9, right associativity) : SP_scope.
-Notation "p & f" := (Branching p f) (at level 60, no associativity) : SP_scope.
+Notation "p '&' c" := (Branching p c) (at level 60, no associativity) : SP_scope.
 Notation "'If' e 'Then' B1 'Else' B2" := (Cond e B1 B2) (at level 60) : SP_scope.
 Notation "'bnil'" := (End) : SP_scope.
 Notation "'nnil'" := (EmptyNet) : SP_scope.
@@ -184,6 +395,50 @@ Check (0!zero; 0?; 1+left; bnil)%SP.
 
 Section SyntacticProperties.
 
+(** ** Syntactic properties *)
+
+(** Equivalence of processes *)
+(* 
+Fixpoint Behaviour_equiv (B1 B2:Behaviour) : Prop :=
+match B1, B2 with
+| bnil%SP, bnil%SP => True
+| Call X, Call Y   => X = Y
+| (p ! e; B)%SP, (p' ! e'; B')%SP => p = p' /\ e = e' /\ Behaviour_equiv B B'
+| (p ? x; B)%SP, (p' ? x'; B')%SP => p = p' /\ x = x' /\ Behaviour_equiv B B'
+| (p (+) l; B)%SP, (p' (+) l'; B')%SP => p = p' /\ l = l' /\ Behaviour_equiv B B'
+| (p & f)%SP, (p' & f')%SP => p = p' /\ (forall l, OptionBehaviour_equiv (f l) (f' l))
+| (If e Then Bt Else Be)%SP, (If e' Then Bt' Else Be')%SP => e = e' /\ Behaviour_equiv Bt Bt' /\ Behaviour_equiv Be Be'
+| _, _ => False
+end
+
+with
+
+OptionBehaviour_equiv (O O':option Behaviour) : Prop :=
+match O, O' with
+| None, None => True
+| Some B, Some B'=> Behaviour_equiv B B'
+| _, _ => False
+end.
+*)
+
+(*
+Definition Behaviour_WF (p:Pid) : Behaviour -> Prop :=
+  Behaviour_rec' _ 
+  True
+  (fun q e B H => p<>q /\ H)
+  (fun q v B H => p<>q /\ H)
+  (fun q l B H => p<>q /\ H)
+  (fun q c H => p<>q /\ forall l B H', (H l B H'))
+  (fun b B1 B2 H1 H2 => H1 /\ H2)
+  (fun X => True).
+*)
+
+(* We probably want a sanity check for Behaviour_WF, comparing it to the commented
+  definition below. *)
+
+(** Well-formedness does not check that, in branchings, all labels are distinct.
+  We might want to add this later. *)
+
 Fixpoint Behaviour_WF (p:Pid) (B:Behaviour) : Prop :=
 match B with
 | bnil%SP => True
@@ -191,99 +446,34 @@ match B with
 | (q ! _; B)%SP => p <> q /\ Behaviour_WF p B
 | (q ? _; B)%SP => p <> q /\ Behaviour_WF p B
 | (q (+) l; B)%SP => p <> q /\ Behaviour_WF p B
-| (q & f)%SP => p <> q /\ (forall l,
-    match (f l) with | Some B' => Behaviour_WF p B' | _ => True end)
+| (q & c)%SP => p <> q /\ fold_right and True (map (fun case => match case with (_, B) => Behaviour_WF p B end) c)
 | (If e Then B1 Else B2)%SP => Behaviour_WF p B1 /\ Behaviour_WF p B2
-end.
-
-Fixpoint B_size (B:Behaviour) :=
-match B with
-| bnil%SP => 0
-| Call _ => 0
-| (_ ! _; B')%SP => 1 + B_size B'
-| (_ ? _; B')%SP => 1 + B_size B'
-| (_ (+) _; B')%SP => 1 + B_size B'
-| (_ & f)%SP =>
-  (match (f left) with | Some B' => B_size B' | _ => 0 end)
-  + (match (f right) with | Some B' => B_size B' | _ => 0 end)
-  + 1
-| (If e Then B1 Else B2)%SP => B_size B1 + B_size B2 + 1
 end.
 
 Lemma Behaviour_WF_dec : forall p B,
   {Behaviour_WF p B} + {~Behaviour_WF p B}.
 Proof.
-assert (forall p p0 B, {Behaviour_WF p B}+{~Behaviour_WF p B} -> {p<>p0 /\ Behaviour_WF p B}+{~(p<>p0 /\ Behaviour_WF p B)}).
-+ intros.
-  elim (P.eq_dec p p0); intro.
-  - right; rewrite a; intro. inversion H0; auto.
-  - inversion_clear H; auto.
-    right; intro. inversion H; auto.
-+ intros.
-  set (n := B_size B).
-  assert (B_size B <= n); auto.
-  clearbody n.
-  revert dependent B.
-  induction n; intros; induction B; simpl in H; simpl; auto with arith;
-    try (exfalso; inversion H; fail).
-  - exfalso.
-    assert (1<=0).
-    2: inversion H0.
-    etransitivity; eauto with arith.
-  - exfalso.
-    inversion H.
-    apply (lt_irrefl 0).
-    eapply lt_le_trans. 2: apply H. auto with arith.
-  - elim (P.eq_dec p p0); intro.
-    1: { right; rewrite a; intro. inversion H0; auto. }
-    revert H; case_eq (o left); case_eq (o right); simpl; intros.
-    * assert (B_size b0 <= n).
-      1: { apply le_S_n. etransitivity.
-           2: apply H1.
-           rewrite plus_comm. auto with arith. }
-      assert (B_size b1 <= n).
-      1: { apply le_S_n. etransitivity.
-           2: apply H1.
-           rewrite plus_comm. auto with arith. }
-      elim (IHn _ H2); elim (IHn _ H3); intros.
-      ++ left; split; auto.
-         induction l; try rewrite H; try rewrite H0; auto.
-      ++ right; intro; inversion_clear H4.
-         generalize (H6 left); rewrite H0; auto.
-      ++ right; intro; inversion_clear H4.
-         generalize (H6 right); rewrite H; auto.
-      ++ right; intro; inversion_clear H4.
-         generalize (H6 left); rewrite H0; auto.
-    * assert (B_size b0 <= n).
-      1: { apply le_S_n. etransitivity.
-           2: apply H1.
-           rewrite plus_comm. auto with arith. }
-      elim (IHn _ H2); intros.
-      ++ left; split; auto.
-         induction l; try rewrite H; try rewrite H0; auto.
-      ++ right; intro; inversion_clear H3.
-         generalize (H5 left); rewrite H0; auto.
-    * assert (B_size b0 <= n).
-      1: { apply le_S_n. etransitivity.
-           2: apply H1.
-           rewrite plus_comm. auto with arith. }
-      elim (IHn _ H2); intros.
-      ++ left; split; auto.
-         induction l; try rewrite H; try rewrite H0; auto.
-      ++ right; intro; inversion_clear H3.
-         generalize (H5 right); rewrite H; auto.
-    * left; split; auto.
-      induction l; try rewrite H; try rewrite H0; auto.
-  - assert (B_size B1 <= S n).
-      1: { etransitivity.
-           2: apply H.
-           auto with arith. }
-    assert (B_size B2 <= S n).
-      1: { etransitivity.
-           2: apply H.
-           auto with arith. }
-    elim IHB1; elim IHB2; intros; auto;
-      right; intro; inversion_clear H2; auto.
+induction B using Behaviour_rec'; simpl; auto;
+  try (elim (P.eq_dec p p0); intro; [idtac | inversion_clear IHB; auto];
+  right; intro H'; inversion_clear H'; auto).
++ assert ({fold_right and True (map (fun case : Label * Behaviour => let (_, B) := case in Behaviour_WF p B) c)} +
+  {~ (fold_right and True (map (fun case : Label * Behaviour => let (_, B) := case in Behaviour_WF p B) c))}).
+  - induction c; simpl; auto.
+    induction a.
+    elim (X a b); simpl; auto.
+    2: right; intro H'; inversion_clear H'; auto.
+    intro.
+    elim IHc; auto.
+    1: right; intro H'; inversion_clear H'; auto.
+    intros. apply X with l; simpl; auto.
+  - elim H.
+    2: right; intro H'; inversion_clear H'; auto.
+    elim (P.eq_dec p p0); auto.
+    right; intro H'; inversion_clear H'; auto.
++ inversion_clear IHB1.
+  2: right; intro H'; inversion_clear H'; auto.
+  inversion_clear IHB2; auto.
+  right; intro H'; inversion_clear H'; auto.
 Qed.
 
 Definition Network_WF (N:Network) : Prop :=
@@ -292,29 +482,22 @@ Definition Network_WF (N:Network) : Prop :=
 Lemma Network_WF_dec : forall ps N, within_ps ps N ->
   {Network_WF N} + {~Network_WF N}.
 Proof.
-intros ps N.
-assert (ps<>nil -> {forall p, In p ps -> Behaviour_WF p (N p)} + {~forall p, In p ps -> Behaviour_WF p (N p)}).
-+ induction ps; simpl.
-  1: right; auto.
-  elim (Behaviour_WF_dec a (N a)); intro.
-  2: right; auto.
-  revert IHps; case ps; intro.
-  * left; intros.
-    inversion_clear H0; [rewrite <- H1; auto | inversion H1].
-  * intros.
-    elim IHps; intros; auto.
-    3: discriminate.
-    1: { left; intros. inversion_clear H0; try rewrite <- H1; auto. }
-    right; intro; auto.
-+ intros.
-  red in H0.
-  case_eq ps; intros.
-  1: { left; intros. red; intros. rewrite H0; try rewrite H1; simpl; auto. }
-  elim H; auto.
-  2: rewrite H1; discriminate.
-  left; red; intros.
-  elim (In_dec P.eq_dec p0 ps); auto.
-  intro; rewrite H0; simpl; auto.
+induction ps; simpl; intros.
++ left; intro; rewrite H; simpl; auto.
++ elim (Behaviour_WF_dec a (N a)); intro.
+  2: right; intro; auto.
+  elim (IHps (Network_rm N a)).
+  3: apply Network_rm_within_ps; auto.
+  - left; intro.
+    case (P.eq_dec p a); intro.
+    1: rewrite e; auto.
+    generalize (a1 p).
+    rewrite <- Pdec.eqb_neq in n.
+    unfold Network_rm. unfold Pid_dec. rewrite n; auto.
+  - right; intro.
+    apply b; intro.
+    unfold Network_rm.
+    case Pid_dec; simpl; auto.
 Qed.
 
 Lemma Par_WF : forall N N', Network_WF N -> Network_WF N' ->
@@ -326,110 +509,32 @@ elim (Behaviour_eq_End_dec (N p)); intro.
 rewrite Par_proj1; auto.
 Qed.
 
-(* FM: we have both B_size and depth, maybe we could use only one. *)
-
-Fixpoint depth (B:Behaviour) : nat :=
-match B with
- | Send p e B' => 1 + depth B'
- | Recv p x B' => 1 + depth B'
- | Sel p l B' => 1 + depth B'
- | Branching p f => 1 +
-    match f left, f right with
-     | Some B1, Some B2 => Nat.max (depth B1) (depth B2)
-     | Some B1, None => depth B1
-     | None, Some B2 => depth B2
-     | None, None => 0
-    end
- | Cond e B1 B2 => 1 + Nat.max (depth B1) (depth B2)
- | Call X => 1
- | End => 1
-end.
-
-Theorem Behaviour_ind_b :
-  forall P : Behaviour -> Prop,
-    P bnil%SP ->
-    (forall (p : Pid) (e : Expr) (b : Behaviour), P b -> P (p ! e; b)%SP) ->
-    (forall (p : Pid) (v : Var) (b : Behaviour), P b -> P (p ? v; b)%SP) ->
-    (forall (p : Pid) (l : Label) (b : Behaviour), P b -> P (p (+) l; b)%SP) ->
-    (forall (p : Pid) (o : Label -> option Behaviour),
-      (forall (b0 : Behaviour), (o left) = Some b0 -> P b0) ->
-      (forall (b1 : Behaviour), (o right) = Some b1 -> P b1) ->
-      P (p & o)%SP
-    ) ->
-    (forall (b : BExpr) (b0 : Behaviour),
-    P b0 -> forall b1 : Behaviour, P b1 -> P (If b Then b0 Else b1)%SP) ->
-    (forall r : RecVar, P (Call r)) -> forall b : Behaviour, P b.
+Lemma WF_Par1 : forall N N', Network_WF (N | N') -> Network_WF N.
 Proof.
-intros.
-revert b.
-assert (forall d b, depth b <= d -> P b).
-2: eauto.
-induction d; intros; case_eq b; intros; auto; rewrite H7 in H6; try (exfalso; inversion H6; fail).
-+ apply H0. apply IHd. simpl in H. auto with arith.
-+ apply H1. apply IHd. simpl in H. auto with arith.
-+ apply H2. apply IHd. simpl in H. auto with arith.
-+ apply H3.
-  (* left branch *)
-  - inversion H6.
-    * intros.
-      rewrite H8 in H9.
-      case_eq (o right); intros; rewrite H10 in H9; apply IHd; rewrite <- H9.
-      ** apply Nat.le_max_l.
-      ** auto with arith.
-    * intros.
-      apply IHd.
-      simpl in H9.
-      rewrite H10 in H9.
-      case_eq (o right); intros.
-      ** rewrite H11 in H9. etransitivity. eapply Nat.le_max_l. eauto with arith.
-      ** rewrite H11 in H9. inversion H9; auto with arith.
-  - inversion H6.
-    * intros.
-      rewrite H8 in H9.
-      case_eq (o left); intros; rewrite H10 in H9; apply IHd; rewrite <- H9; auto with arith.
-      apply Nat.le_max_r.
-    * intros.
-      apply IHd.
-      simpl in H9.
-      rewrite H10 in H9.
-      case_eq (o left); intros.
-      ** rewrite H11 in H9. etransitivity. eapply Nat.le_max_r. eauto with arith.
-      ** rewrite H11 in H9. inversion H9; auto with arith.
-+ apply H4; apply IHd; simpl in H; apply le_S_n in H6.
-  - etransitivity. eapply Nat.le_max_l. eauto.
-  - etransitivity. eapply Nat.le_max_r. eauto.
+intros; intro.
+elim (Behaviour_eq_End_dec (N p)); intro.
+1: rewrite a; simpl; auto.
+rewrite <- (Par_proj1 N N'); auto.
 Qed.
 
-(*
-Definition Program_WF (P:Program) := 
-  (forall X p, Behaviour_WF p (Procedures P X)) /\
-  (forall p, Network_WF (Net p)).
-
- add within_Xs and decidability *)
-
-(* WF program doesn't make sense.
-   But: program with WF network reduces to program with WF network is
-   an interesting property that is guaranteed by EPP. *)
-
-End SyntacticProperties.
-
-Section Semantics.
+Lemma WF_Par2 : forall N N', Network_disjoint N N' ->
+  Network_WF (N | N') -> Network_WF N'.
+Proof.
+intros; intro.
+elim (Behaviour_eq_End_dec (N' p)); intro.
+1: rewrite a; simpl; auto.
+rewrite <- (Par_proj2 N N'); auto.
+elim (Behaviour_eq_End_dec (N p)); auto.
+intro; exfalso.
+elim (H p); auto.
+Qed.
 
 Lemma Network_WF_par : forall N N', Network_disjoint N N' ->
   Network_WF (N | N') -> Network_WF N /\ Network_WF N'.
 Proof.
-intros.
-split; intro.
-+ elim (Behaviour_eq_End_dec (N p)); intro.
-  1: rewrite a; simpl; auto.
-  rewrite <- (Par_proj1 N N'); auto.
-+ elim (Behaviour_eq_End_dec (N' p)); intro.
-  1: rewrite a; simpl; auto.
-  rewrite <- (Par_proj2 N N'); auto.
-  elim (Behaviour_eq_End_dec (N p)); auto.
-  intro.
-  exfalso.
-  elim (H p); auto.
+split.
+apply WF_Par1 with N'; auto.
+apply WF_Par2 with N; auto.
 Qed.
 
 Lemma Network_WF_comm : forall N N', Network_disjoint N N' ->
@@ -440,43 +545,54 @@ elim (Network_WF_par N N'); intros; auto.
 apply Par_WF; auto.
 Qed.
 
+(* WF program doesn't make sense, because procedures don't know the processes
+  that will execute them, so we do not know what to pass to Behaviour_WF.
+   But: program with WF network reduces to program with WF network is
+   an interesting property that is guaranteed by EPP. *)
+
+End SyntacticProperties.
+
+Section Semantics.
+
 Definition Network_eq_upTo (N:Network) ps N' : Prop :=
   forall p, ~In p ps -> N' p = N p.
 
 Inductive SP_To (Procs : RecVar -> Behaviour) :
-  Network -> State -> TransitionLabel -> Network -> State -> Prop :=
- | S_Com N N' s p e q x B B':
+  Network -> State -> RichLabel -> Network -> State -> Prop :=
+ | S_Com N p e B q x B' N' s s' :
     N p = (q ! e ; B)%SP -> N q = (p ? x ; B')%SP ->
-    N' p = B -> N' q = B' ->
-    Network_eq_upTo N (p::q::List.nil) N' ->
     let v := (eval_on_state e s p) in
-    SP_To Procs N s (L_Com p v q) N' (update s q x v)
- | S_Sel N N' s p q l B f B':
-    N p = (q (+) l ; B)%SP -> N q = (p & f)%SP ->
-    f l = Some B' ->
-    N' p = B -> N' q = B' ->
-    Network_eq_upTo N (p::q::nil) N' ->
-    SP_To Procs N s (L_Sel p q l) N' s
- | S_Then N N' s p b B1 B2 :
+    Network_eq N' ((Network_rm (Network_rm N p) q) | p[B] | q[B']) ->
+    eq_state_ext s' (update s q x v) ->
+    SP_To Procs N s (R_Com p v q x) N' s'
+ | S_Sel N p l B q c B' N' s s' :
+    N p = (q (+) l ; B)%SP -> N q = (p & c)%SP -> In (l, B') c ->
+    Network_eq N' ((Network_rm (Network_rm N p) q) | p[B] | q[B']) ->
+    eq_state_ext s s' ->
+    SP_To Procs N s (R_Sel p q l) N' s'
+ | S_Then N p b B1 B2 N' s s' :
     N p = (If b Then B1 Else B2)%SP ->
-    N' p = B1 -> (beval_on_state b s p = true) ->
-    Network_eq_upTo N (p::nil) N' ->
-    SP_To Procs N s (L_Tau p) N' s
- | S_Else N N' s p b B1 B2 :
+    beval_on_state b s p = true ->
+    Network_eq N' ((Network_rm N p) | p[B1]) ->
+    eq_state_ext s s' ->
+    SP_To Procs N s (R_Cond p) N' s'
+ | S_Else N p b B1 B2 N' s s' :
     N p = (If b Then B1 Else B2)%SP ->
-    N' p = B2 -> (beval_on_state b s p = false) ->
-    Network_eq_upTo N (p::nil) N' ->
-    SP_To Procs N s (L_Tau p) N' s
- | S_Call N N' s p X :
-    N p = Call X -> N' p = Procs X ->
-    Network_eq_upTo N (p::nil) N' ->
-    SP_To Procs N s (L_Tau p) N' s.
+    beval_on_state b s p = false ->
+    Network_eq N' ((Network_rm N p) | p[B2]) ->
+    eq_state_ext s s' ->
+    SP_To Procs N s (R_Cond p) N' s'
+ | S_Call N p X N' s s' :
+    N p = Call X ->
+    Network_eq N' ((Network_rm N p) | p[Procs X]) ->
+    eq_state_ext s s' ->
+    SP_To Procs N s (R_Call X p) N' s'.
 
 Definition Configuration : Type := Program * State.
 
 Inductive SPP_To : Configuration -> TransitionLabel -> Configuration -> Prop :=
  | SPP_To_intro Procs N s t N' s' : SP_To Procs N s t N' s' ->
-     SPP_To (Build_Program Procs N,s) t (Build_Program Procs N',s').
+     SPP_To (Build_Program Procs N,s) (forget t) (Build_Program Procs N',s').
 
 Inductive SPP_ToStar : Configuration -> list TransitionLabel -> Configuration -> Prop :=
  | SPT_Refl c : SPP_ToStar c nil c
